Fix proof of Alpha for full expressions.

Alpha.v
@@ -1,23 +1,25 @@
-Require Import Util Map Env EnvTy Exp IL ParamsMatch AllInRel Sim.
+Require Import Util Map Env EnvTy Exp IL ParamsMatch AllInRel Sim Computable.
 
 Import F.
 
 Set Implicit Arguments.
+Unset Printing Records.
 
 Inductive alpha : env var -> env var -> stmt -> stmt -> Prop :=
-| alpha_return ra ira x y 
-  : ra x = y -> ira y = x -> alpha ra ira (stmtReturn x) (stmtReturn y)
+| alpha_return ra ira e e' 
+  : alpha_exp ra ira e e'  -> alpha ra ira (stmtReturn e) (stmtReturn e')
 | alpha_goto ra ira l X Y 
-  : lookup_list ra X = Y -> lookup_list ira Y = X 
-  -> alpha ra ira (stmtGoto l X) (stmtGoto l Y)
+  : length X = length Y
+    -> (forall n x y, get X n x -> get Y n y -> alpha_exp ra ira x y)
+    -> alpha ra ira (stmtGoto l X) (stmtGoto l Y)
 | alpha_assign ra ira x y e e' s s' 
   : alpha_exp ra ira e e' 
   -> alpha (ra[x<-y]) (ira[y <- x]) s s' -> alpha ra ira (stmtExp x e s) (stmtExp y e' s')
-| alpha_if ra ira x y s s' t t' 
-  : ra x = y -> ira y = x 
+| alpha_if ra ira e e' s s' t t' 
+  : alpha_exp ra ira e e'
   -> alpha ra ira s s'
   -> alpha ra ira t t'
-  -> alpha ra ira (stmtIf x s t) (stmtIf y s' t')
+  -> alpha ra ira (stmtIf e s t) (stmtIf e' s' t')
 | alpha_let ra ira s s' Z Z' t t'
   : length Z = length Z'
   -> alpha (ra [ Z <-- Z']) (ira [ Z' <-- Z ]) s s' 
@@ -25,49 +27,72 @@ Inductive alpha : env var -> env var -> stmt -> stmt -> Prop :=
  
 Global Instance alpha_morph 
  : Proper (feq ==> feq ==> eq ==> eq ==> impl) alpha.
-Proof. 
+Proof.  
   unfold respectful, Proper, impl; intros; subst.
-  general induction H3; econstructor; eauto;
-  try (now rewrite <- H1; eauto);
-  try (now rewrite <- H2; eauto).
-  eapply alpha_exp_morph; eauto.
-  eapply IHalpha. rewrite H0. reflexivity.
-  rewrite H1; reflexivity.
-  eapply IHalpha1. rewrite H0; reflexivity. 
-  rewrite H1; reflexivity.
+  general induction H3; econstructor; eauto using alpha_exp_morph.
+  - eapply IHalpha. 
+    + rewrite H0; reflexivity.
+    + rewrite H1; reflexivity.
+  - eapply IHalpha1.
+    + rewrite H0; reflexivity.
+    + rewrite H1; reflexivity.
 Qed.
 
 Lemma alpha_refl s
   : alpha id id s s.
 Proof.
-  general induction s; eauto using alpha. 
-  econstructor. eapply alpha_exp_refl.
-  rewrite update_id; eauto.
-  econstructor; eauto using lookup_id.
-
-  econstructor; try rewrite update_with_list_id; eauto using length_eq_refl.
+  general induction s; eauto using alpha, alpha_exp_refl. 
+  - econstructor. eapply alpha_exp_refl.
+    rewrite update_id; eauto.
+  - constructor; eauto using lookup_id.
+    + intros. get_functional; subst; eauto using alpha_exp_refl.
+  - econstructor; try rewrite update_with_list_id; eauto using length_eq_refl.
 Qed.
   
 Lemma alpha_sym ϱ ϱ' s s'
   : alpha ϱ ϱ' s s'
   ->alpha ϱ' ϱ s' s.
 Proof.
-  intros. general induction H; eauto using alpha, length_eq_sym.
-  econstructor. eapply alpha_exp_sym. eauto. eauto.
+  intros. general induction H; eauto using alpha, length_eq_sym, alpha_exp_sym.
 Qed.
+
+Lemma list_union_get {X} `{OrderedType X} L (x:X) u
+: x ∈ fold_left union L u
+  -> { n : nat & { t : set X | get L n t /\ x ∈ t} } + { x ∈ u }.
+Proof.
+  intros. general induction L; simpl in *; eauto.
+  - decide (x ∈ a).
+    + left; do 2 eexists; split; eauto using get.
+    + edestruct IHL as [[? []]|]; eauto; dcr.
+      * left. eauto using get.
+      * right. cset_tac; intuition.
+Qed.
+
+
+Lemma get_list_union_map X Y `{OrderedType Y} (f:X -> set Y) L n x
+: get L n x
+  -> f x [<=] list_union (List.map f L).
+Proof.
+  intros. eapply incl_list_union. 
+  + eapply map_get_1; eauto. 
+  + reflexivity.
+Qed.
+
 
 Lemma alpha_inverse_on  ϱ ϱ' s t
   : alpha ϱ ϱ' s t -> inverse_on (freeVars s) ϱ ϱ'. 
 Proof.
-  intros A. general induction A; simpl.
-  + hnf; intros. cset_tac. rewrite H1. congruence.
-  + eapply lookup_list_inverse_on; try intuition.
-    rewrite H. rewrite H0. eauto.
+  intros A. general induction A; simpl; eauto using alpha_exp_inverse_on.
+  + hnf; intros.
+    edestruct (list_union_get (List.map Exp.freeVars X)) as [[? []]|]; eauto; dcr.
+    edestruct map_get_4; eauto; dcr. 
+    edestruct get_length_eq; eauto. subst.
+    eapply alpha_exp_inverse_on; eauto. 
+    inv i.
   + hnf; intros. cset_tac. destruct H0; dcr.
     specialize (IHA x0 H1). lud.
     eapply alpha_exp_inverse_on; eauto.
-  + eapply inverse_on_union. eapply inverse_on_union; eauto.
-    hnf; intros; cset_tac. rewrite H1. congruence.
+  + eapply inverse_on_union; try eapply inverse_on_union; eauto using alpha_exp_inverse_on.
   + eapply inverse_on_union; eauto.
     eapply update_with_list_inverse_on; eauto.
 Qed.
@@ -78,17 +103,18 @@ Lemma alpha_agree_on_morph f g ϱ ϱ' s t
   -> agree_on (freeVars s) f ϱ
   -> alpha f g s t.
 Proof. 
-  intros. general induction H; eauto; simpl in * |- *.
-  + econstructor. rewrite H2; eauto. cset_tac; eauto.
-    rewrite H1; eauto. eapply lookup_set_spec. intuition. eexists x; cset_tac; eauto.
-  + econstructor. erewrite lookup_list_agree; eauto.
-    erewrite lookup_list_agree; eauto. rewrite <- H. rewrite of_list_lookup_list; eauto. 
-    intuition.
-  + econstructor. eapply alpha_exp_agree_on_morph; eauto.
-    eapply agree_on_incl; eauto. eapply lookup_set_incl; eauto. intuition.
-    eapply union_subset_2. eapply agree_on_incl; eauto.
-    eapply union_subset_2.
-    eapply IHalpha; eauto. 
+  intros. general induction H; simpl in * |- *; eauto using alpha, alpha_exp_agree_on_morph.
+  + econstructor; intros; eauto.
+    eapply alpha_exp_agree_on_morph; eauto.
+    eapply agree_on_incl; eauto. 
+    eapply lookup_set_incl; try now intuition; eauto using get_list_union_map.
+    eapply agree_on_incl; eauto using get_list_union_map.
+  + econstructor.
+    eapply alpha_exp_agree_on_morph; eauto.
+    eapply agree_on_incl; eauto.
+    eapply lookup_set_incl; try now intuition; eauto using get_list_union_map.
+    eapply agree_on_incl; eauto. cset_tac; intuition.
+    eapply IHalpha; eauto.
     - eapply agree_on_update_same. eapply agree_on_incl; eauto.
       hnf; intros. eapply lookup_set_spec. intuition.
       cset_tac; eqs. eapply lookup_set_spec in H4.
@@ -96,9 +122,11 @@ Proof.
       split; eqs. cset_tac. left. split; eauto. intuition.
     - eapply agree_on_update_same. eapply agree_on_incl; eauto.
       cset_tac; eqs; intuition. 
-  + econstructor; eauto. rewrite H4; eauto. cset_tac; intuition.
-    rewrite H3; eauto. eapply lookup_set_spec; try intuition.
-    eexists x; cset_tac; intuition.
+  + econstructor; eauto. 
+    - eapply alpha_exp_agree_on_morph; eauto.
+      eapply agree_on_incl; eauto. 
+      eapply lookup_set_incl; try now intuition; eauto using get_list_union_map.
+      eapply agree_on_incl; eauto using get_list_union_map. cset_tac; intuition.
     - eapply IHalpha1. eapply agree_on_incl; eauto.
       eapply lookup_set_incl; intuition.
       cset_tac; intuition. 
@@ -134,55 +162,53 @@ Lemma alpha_inverse_on_agree f g ϱ ϱ' s t
 Proof. 
   intros. eapply alpha_agree_on_morph; eauto.
   symmetry in H1.
-  eapply inverse_on_agree_on_2; eauto. 
-  intuition. intuition. intuition. intuition.
+  eapply inverse_on_agree_on_2; eauto; try now intuition.
   eapply inverse_on_agree_on; eauto; try intuition.
   eapply alpha_inverse_on in H.
   eapply inverse_on_agree_on; try eassumption; try intuition.
   eapply inverse_on_agree_on_2; eauto; try intuition.
 Qed.
 
+Ltac invt ty :=
+  match goal with 
+      | h: ty |- _ => inv h
+      | h: ty _ |- _ => inv h
+      | h: ty _ _ |- _ => inv h
+      | h: ty _ _ _ |- _ => inv h
+      | h: ty _ _ _ _ |- _ => inv h
+      | h: ty _ _ _ _ _ |- _ => inv h
+  end.
+
 Lemma alpha_trans ϱ1 ϱ1' ϱ2 ϱ2' s s' s''
   : alpha ϱ1 ϱ1' s s' -> alpha ϱ2 ϱ2' s' s'' -> alpha (ϱ1 ∘ ϱ2) (ϱ2' ∘ ϱ1') s s''.
 Proof.
-  intros. general induction H. 
-  + inversion H1. econstructor; subst y0 y; eauto. unfold comp. rewrite H6. congruence.
-  + inversion H1. econstructor; rewrite comp_lookup_list; try rewrite H; try rewrite H8; eauto.
-  + inversion H1. econstructor; eauto. eapply alpha_exp_trans; eauto.
-    subst x0 s0 e0 ra0 ira0 s''.
+  intros. general induction H; invt alpha; eauto using alpha_exp_trans, alpha. 
+  + econstructor; eauto. etransitivity; eauto.
+    intros. edestruct (get_length_eq _ H2 H); eauto. 
+    eapply alpha_exp_trans; eauto.
+  + econstructor; eauto using alpha_exp_trans.
     specialize (IHalpha _ _ _ H9).
     eapply alpha_inverse_on in H0.
     eapply alpha_inverse_on_agree; eauto. 
     eapply inverse_on_comp; eauto. eapply alpha_inverse_on; eauto.
     symmetry. eapply lookup_set_agree_on_comp. intuition.
     eapply inverse_on_update_lookup_set. intuition. eauto.
-  + inversion H3. subst ra0 ira0 x0 s0 t0 s''. econstructor.
-    unfold comp. congruence. unfold comp. congruence.
-    eapply IHalpha1; eauto. eapply IHalpha2; eauto.
-  + inversion H2. subst ra0 ira0 Z0 s0 t0 s''.
-    econstructor. congruence. 
+  + econstructor; eauto. congruence. 
     specialize (IHalpha1 _ _ _ H10).
     eapply alpha_inverse_on_agree; eauto.
     eapply alpha_inverse_on in IHalpha1.
     pose proof (inverse_on_comp_list _ _ _ H H8 IHalpha1).
-    pose proof (inverse_on_sym IHalpha1); try (now intuition).
+    pose proof (inverse_on_sym IHalpha1).
     pose proof H3.
-    eapply inverse_on_comp_list in H4; try (now intuition); eauto.
-    eapply inverse_on_agree_on; eauto; try intuition.
-    
+    eapply inverse_on_comp_list in H4; eauto.
+    eapply inverse_on_agree_on; eauto.
     symmetry. eapply inverse_on_comp_list; eauto.
-    intuition. intuition. instantiate (1:=ira). intuition.
-    instantiate (1:=ϱ2'). intuition. eapply alpha_inverse_on; eauto.
-    
-    eapply IHalpha2; eauto.
+    instantiate (1:=ira).
+    instantiate (1:=ϱ2'). eapply alpha_inverse_on; eauto.
 Qed.
-
-
-
 
 Definition envCorr ra ira (E E':env val) :=
   forall x y, ra x = y -> ira y = x -> E x = E' y.
-
 
 Lemma envCorr_idOn_refl (E:env val)
   : envCorr id id E E.
@@ -237,6 +263,21 @@ Proof.
   eapply envCorr_update; eauto.
 Qed.
 
+Lemma envCorr_update_list bra bira block_E block_E' block_Z block_Z' ra ira
+  E E' vl (EC':envCorr ra ira E E')
+  (EC: envCorr bra bira block_E block_E')
+  (LC: length block_Z = length block_Z')
+  (LC': length block_Z = length vl)
+  : envCorr (bra [ block_Z <-- block_Z' ]) (bira [ block_Z' <-- block_Z ])
+  (block_E  [ block_Z <-- vl ])
+  (block_E' [ block_Z' <-- vl ]).
+Proof.
+  eapply length_length_eq in LC.
+  eapply length_length_eq in LC'.
+  general induction LC; inv LC'; simpl; eauto.
+  eapply envCorr_update; eauto.
+Qed.
+
 Lemma alpha_exp_eval : forall ra ira e e' E E',
   alpha_exp ra ira e e' -> 
   envCorr ra ira E E' -> 
@@ -262,41 +303,37 @@ Proof.
   revert σ1 σ2; cofix; intros.
   destruct H; inversion AE; subst ra0 ira0; simpl in * |- *;
   try subst s s'; simpl in * |- *.
-  + eapply simE; try eapply star_refl; simpl; try stuck.
-    erewrite EC; eauto.
-  + assert (length X = length Y). {
-      rewrite <- H. rewrite lookup_list_length; eauto.
-    }
-    destruct (get_dec L (counted l)) as [[[Eb Zb sb]]|]; [| try no_step].
-    decide (length Zb = length Y); [| try no_step].
-    provide_invariants_3. subst x1 x x0 x2 ; simpl in *.
-    one_step; simpl; try congruence; eauto.
-    simpl. eapply alphaSim_sim; econstructor; eauto. 
-    eapply envCorr_update_lists; eauto; congruence.
-    clear H H0; no_step. get_functional; subst; simpl in *; congruence.
-    provide_invariants_3; simpl in *; congruence.
-    clear H H0; no_step; provide_invariants_3; eauto.
+  + eapply simE; try eapply star_refl; simpl; eauto using alpha_exp_eval; try stuck.
+  + destruct (get_dec L (counted l)) as [[[Eb Zb sb]]|].
+    decide (length Zb = length Y).
+    case_eq (omap (exp_eval E) X); intros.
+    - provide_invariants_3. simpl in *.
+      one_step; simpl; try congruence; eauto.
+      erewrite omap_agree_2; eauto. intros. symmetry.
+      eapply alpha_exp_eval. eapply H0; eauto; eauto. hnf; intros; eauto.
+      simpl. eapply alphaSim_sim; econstructor; eauto. 
+      eapply envCorr_update_list; eauto. exploit omap_length; eauto. congruence.
+    - no_step. erewrite omap_agree_2 in H1; try eapply H.
+      erewrite H1 in def. congruence.
+      intros. eapply alpha_exp_eval. eapply H0; eauto. eauto.
+    - provide_invariants_3; simpl in *. no_step. simpl in *. 
+      get_functional; subst. simpl in *. congruence.
+      get_functional; subst. simpl in *. congruence.
+    - no_step; eauto. provide_invariants_3; eauto.
   + case_eq (exp_eval E e); intros.
-    eapply simS; try eapply plusO. 
-    econstructor; eauto. 
-    econstructor; eauto. instantiate (1:=v).
-    erewrite <- alpha_exp_eval; eauto.
+    one_step. erewrite <- alpha_exp_eval; eauto.
     eapply alphaSim_sim; econstructor; eauto using envCorr_update.
     eapply simE; try eapply star_refl; eauto; stuck.
     erewrite alpha_exp_eval in H1; eauto. congruence.
-  + case_eq (val2bool (E x)); intros. 
-    eapply simS; try eapply plusO.
-    econstructor; eauto.
-    econstructor; eauto. erewrite <- EC; eauto.
+  + case_eq (exp_eval E e); intros.
+    case_eq (val2bool v); intros. 
+    one_step. erewrite <- alpha_exp_eval; eauto.
     eapply alphaSim_sim; econstructor; eauto.
-    eapply simS; try eapply plusO.
-    eapply F.stepIfF; eauto.
-    eapply F.stepIfF; eauto. erewrite <- EC; eauto.
+    one_step. erewrite <- alpha_exp_eval; eauto.
     eapply alphaSim_sim; econstructor; eauto.
-  + eapply simS; try eapply plusO.
-    econstructor; eauto.
-    econstructor; eauto.
-    eapply alphaSim_sim.
+    no_step; erewrite <- alpha_exp_eval in def; eauto. 
+    congruence. congruence.
+  + one_step. eapply alphaSim_sim.
     econstructor; eauto.
     econstructor; eauto. econstructor; eauto.
 Qed.
